\documentclass{article}
\usepackage[utf8]{inputenc}
\usepackage[english]{babel}
\usepackage[]{amsthm} %lets us use \begin{proof}
\usepackage[]{amssymb} %gives us the character \varnothing
\usepackage[]{amsmath}
\usepackage[parfill]{parskip} %avoid indent when skipping lines
\usepackage[toc,page]{appendix}
\usepackage{mathtools}
\usepackage{hyperref}
\hypersetup{
	colorlinks=true,
	linkcolor=blue,
	filecolor=magenta,      
	urlcolor=cyan,
	pdftitle={18.100A-ps12},
	pdfpagemode=FullScreen,
}
%\urlstyle{same}
\newcommand{\R}{\mathbb{R}} %the real numbers
\newcommand{\N}{\mathbb{N}} %the natural numbers
\newcommand{\M}{\mathcal{M}} %set of all Lebesgue-measurable sets
\newcommand{\Q}{\mathbb{Q}} % the rational numbers

\title{18.100A Assignment 12}
\author{Octavio Vega}
\date\today

\begin{document}
\maketitle
	
\section*{Problem 1}
\subsection*{(a)}
\begin{proof}
	Suppose $\exists c \in [a, b]$ such that $f(c) > 0$. Since $f$ is continuous, $\exists \delta > 0$ such that if $|x - c| < \delta$, then $|f(x) - f(x)| < \frac{f(c)}{2}$, i.e. $\frac{f(c)}{2} < f(x)$. We compute
	\begin{align}
		0 &> \int_a^b f \\
		&> \int_a ^b \frac{f(c)}{2} \\
		&= \frac{f(c)}{2}(b - a) \\
		&> 0,
	\end{align}
	i.e. $0 > 0$ $(\Rightarrow \Leftarrow)$, which is cleary a contradiction.
	
	Therefore $f(x) = 0$ $\forall x \in [a, b]$.  
\end{proof}

\subsection*{(b)}
\begin{proof}
	Let $E = \int_a ^b (u')^2 \mathrm{d}x$. Then $E \geq 0$ since $(u')^2 \geq 0$. Using integration by parts, we have
	\begin{align}
		E &= \int_a ^b u' u' \mathrm{d}x \\
		&= u u' \big |_a ^b - \int_a ^b u u'' \mathrm{d}x \\
		&= u'(b) u(b) - u'(a) u(a) - \int_a ^b u (V u) \mathrm{d}x \\
		&= - \int_a ^b V u^2 \mathrm{d}x.
	\end{align}
	But $V(x) \geq 0$ and $u^2 \geq 0$, so $-(Vu^2) \leq 0$, hence $E \leq 0$. Thus $E = 0$, which must mean that 
	\begin{equation}
		\int_a ^b (u')^2 \mathrm{d}x = 0,
	\end{equation}
	and by part \textbf{(a)}, this implies that $(u')^2 = 0$  $\forall x \in [a, b]$. Hence $u'(x) = 0$ for all $x$, and since $u(a) = 0$, then $u$ remains constant at $0$; i.e. $u = 0$ everywhere.
\end{proof}
	
\end{document}