\documentclass{article}
\usepackage[utf8]{inputenc}
\usepackage[english]{babel}
\usepackage[]{amsthm} %lets us use \begin{proof}
\usepackage[]{amssymb} %gives us the character \varnothing
\usepackage[]{amsmath}
\usepackage[parfill]{parskip} %avoid indent when skipping lines

\title{18.100A Assignment 2}
\author{Octavio Vega}
\date\today

\begin{document}
\maketitle
	
\section*{Problem 1}
\begin{proof}
	(By contradiction).
	
	Suppose instead that $xy \leq xz$. Then
	
	$\implies xy - xz \leq 0$
	
	$\implies x(y-z) \leq 0$.
	
	Since $x<0$ by assumption, it must then be true that $y-z\geq 0$. But then
	
	$\implies y \geq z \quad \Rightarrow\Leftarrow$,
	
	which is a contradiction since we assumed that $y<z$. Thus, $xy>xz$.
\end{proof}
	
\end{document}